LogicalRefinement/Stlc/InterpIrrel.lean
@@ -13,10 +13,18 @@ def Context.is_irrel (Γ: Context) (n: Nat): Prop
 def Context.is_rel (Γ: Context) (n: Nat): Prop
   := ∃A, HasVar Γ n (HypKind.val type) A
 
+def Context.is_val (Γ: Context) (n: Nat): Prop
+  := ∃A s, HasVar Γ n (HypKind.val s) A
+
 @[simp] def Stlc.Context.interp.eq_mod_lrt 
   {Γ' Δ': Stlc.Context} (G: Γ'.interp) (D: Δ'.interp) 
   (Γ Δ: _root_.Context): Prop
   := ∀n: Nat, Γ.is_rel n ∧ Δ.is_rel n -> eq_at G D n
+
+@[simp] def Stlc.Context.interp.eq_mod_lrt_val 
+  {Γ' Δ': Stlc.Context} (G: Γ'.interp) (D: Δ'.interp) 
+  (Γ Δ: _root_.Context): Prop
+  := ∀n: Nat, Γ.is_val n ∧ Δ.is_val n -> eq_at G D n
 
 theorem Stlc.Context.interp.eq_mod_lrt.extend
     {Γ' Δ': Stlc.Context} 
@@ -36,6 +44,30 @@ theorem Stlc.Context.interp.eq_mod_lrt.extend
       constructor
       constructor
       assumption
+      constructor
+      assumption
+  }
+
+theorem Stlc.Context.interp.eq_mod_lrt_val.extend
+    {Γ' Δ': Stlc.Context} 
+    {H: Hyp} {x: Option H.ty.stlc_ty.interp} 
+    {G: Γ'.interp} {D: Δ'.interp} {Γ Δ: _root_.Context}:
+  G.eq_mod_lrt_val D Γ Δ -> 
+  @eq_mod_lrt_val (_::Γ') (_::Δ') (x, G) (x, D) (H::Γ) (H::Δ)
+  := by {
+    intro HGG' n Hn;
+    cases n with
+    | zero => exact ⟨rfl, rfl⟩
+    | succ n => 
+      apply HGG' n;
+      have ⟨⟨A, s, HAn⟩, ⟨A', s', HAn'⟩⟩ := Hn;
+      cases HAn;
+      cases HAn';
+      constructor
+      constructor
+      constructor
+      assumption
+      constructor
       constructor
       assumption
   }
@@ -89,11 +121,43 @@ theorem Stlc.Context.interp.eq_mod_lrt.extend_gst
       constructor
       assumption
   }
+  
+theorem Stlc.Context.interp.eq_mod_lrt_val.extend_gst
+    {Γ' Δ': Stlc.Context} 
+    {A: Term} {x y: Option A.stlc_ty.interp} 
+    {G: Γ'.interp} {D: Δ'.interp} {Γ Δ: _root_.Context}:
+  G.eq_mod_lrt_val D Γ Δ -> 
+  @eq_mod_lrt_val (_::Γ') (_::Δ') (x, G) (y, D) ((Hyp.mk A HypKind.gst)::Γ) ((Hyp.mk A HypKind.gst)::Δ)
+  := by {
+    intro HGG' n Hn;
+    cases n with
+    | zero =>
+      have ⟨⟨_, _, HA⟩, _⟩ := Hn;
+      cases HA with
+      | zero Hk => cases Hk
+    | succ n => 
+      apply HGG' n;
+      have ⟨⟨A, s, HAn⟩, ⟨A', s', HAn'⟩⟩ := Hn;
+      cases HAn;
+      cases HAn';
+      constructor
+      constructor
+      constructor
+      assumption
+      constructor
+      constructor
+      assumption
+  }
 
 
 theorem Stlc.Context.interp.eq_mod_lrt_refl
     {Γ': Stlc.Context} (G: Γ'.interp) (Γ Δ: _root_.Context):
     G.eq_mod_lrt G Γ Δ
+  := λn _ => G.eq_at_refl n 
+
+theorem Stlc.Context.interp.eq_mod_lrt_val_refl
+    {Γ': Stlc.Context} (G: Γ'.interp) (Γ Δ: _root_.Context):
+    G.eq_mod_lrt_val G Γ Δ
   := λn _ => G.eq_at_refl n 
 
 theorem Stlc.Context.interp.eq_mod_lrt_downgrade
@@ -136,117 +200,188 @@ theorem Stlc.Context.interp.eq_mod_lrt_downgrade
           )
   } 
 
-theorem HasType.interp_irrel_dep {Γ a A} 
-  (H: Γ ⊢ a: expr type A) (n: Nat)
-  (Ha: a.stlc.has_dep n): Γ.is_rel n := by {
-    generalize HA': expr type A = A';
+theorem Stlc.Context.interp.eq_mod_lrt_val_downgrade
+    {Γ: _root_.Context} (G: Γ.upgrade.stlc.interp) (Δ) :
+    G.downgrade.eq_mod_lrt_val G Γ Δ
+  := by {
+    induction Γ generalizing Δ with
+    | nil => intro _ ⟨⟨_, _, HΓ⟩, _⟩; cases HΓ
+    | cons H Γ I =>
+      intro n ⟨⟨A, _, HΓ⟩, ⟨B, _, HΔ⟩⟩;
+      cases n with
+      | zero => 
+        cases H with
+        | mk A k =>
+          cases k with
+          | val s => exact ⟨rfl, rfl⟩
+          | gst => cases HΓ with | zero Hk => cases Hk
+      | succ n =>
+        cases H with
+        | mk A k =>
+          cases k <;> (
+            cases G;
+            unfold eq_at;
+            simp only [
+              Context.upgrade, Context.stlc, Hyp.upgrade,
+              downgrade
+            ]
+            cases HΓ;
+            cases HΔ;
+            apply I;
+            constructor
+            constructor
+            constructor
+            assumption
+            constructor
+            constructor
+            assumption
+          )
+  } 
+
+theorem HasType.interp_irrel_dep_cast {Γ a A n}
+  (H: Γ ⊢ a: expr type A) (Ha: a = Term.var n ∨ Γ.is_rel n): Γ.is_rel n
+  := by {
+    cases Ha with
+    | inl Ha => rw [Ha] at H; cases H; exact ⟨_, by assumption⟩
+    | inr Ha => exact Ha
+  }
+
+theorem HasType.interp_irrel_dep {Γ a s A} 
+  (H: Γ ⊢ a: expr s A) (n: Nat)
+  (Ha: a.stlc.has_dep n): a = Term.var n ∨ Γ.is_rel n := by {
+    generalize HA': expr s A = A';
     rw [HA'] at H;
-    induction H generalizing A n with
-    | var HA Hv _IA =>
-      cases Ha; 
-      cases HA';
-      exact ⟨_, Hv⟩
-    | lam _ _ Is _ => 
-      cases Is (n + 1) Ha rfl with
+    induction H generalizing A s n with
+    | var => cases Ha; exact Or.inl rfl
+    | lam Hs _ Is _ => 
+      apply Or.inr
+      cases Hs.interp_irrel_dep_cast (Is (n + 1) Ha rfl) with
       | intro A Hv => 
         cases Hv;
         exact ⟨_, by assumption⟩
-    | app _ _ _ _ Il Ir => 
+    | app _ Hl Hr _ Il Ir => 
+      apply Or.inr
       cases Ha with
-      | inl Ha => exact Il n Ha rfl
-      | inr Ha => exact Ir n Ha rfl
-    | pair _ _ _ _ Il Ir => 
+      | inl Ha => exact Hl.interp_irrel_dep_cast (Il n Ha rfl)
+      | inr Ha => exact Hr.interp_irrel_dep_cast (Ir n Ha rfl)
+    | pair _ Hl Hr _ Il Ir => 
+      apply Or.inr
       cases Ha with
-      | inl Ha => exact Il n Ha rfl
-      | inr Ha => exact Ir n Ha rfl
-    | let_pair _ _ _ _ _ Ie _ _ _ Ie' => 
+      | inl Ha => exact Hl.interp_irrel_dep_cast (Il n Ha rfl)
+      | inr Ha => exact Hr.interp_irrel_dep_cast (Ir n Ha rfl)
+    | let_pair He _ _ _ He' Ie _ _ _ Ie' => 
+      apply Or.inr
       cases HA';
+      rename AnnotSort => k;
+      cases k;
+      case prop => 
+        dsimp only [Stlc.has_dep, Term.stlc] at Ha;
       cases Ha with
-      | inl Ha => exact Ie n Ha rfl
+      | inl Ha => exact He.interp_irrel_dep_cast (Ie n Ha rfl)
       | inr Ha => 
-        cases Ie' (n + 2) Ha rfl with
+        cases He'.interp_irrel_dep_cast (Ie' (n + 2) Ha rfl) with
         | intro A Hv =>
           cases Hv with
           | succ Hv => 
             cases Hv;
             exact ⟨_, by assumption⟩
-    | inj_l _ _ Ie _ => exact Ie n Ha rfl
-    | inj_r _ _ Ie _ => exact Ie n Ha rfl
-    | case _ _ _ _ _ _ Id _ _ _ Il Ir => 
+    | inj_l He _ Ie _ => exact Or.inr (He.interp_irrel_dep_cast (Ie n Ha rfl))
+    | inj_r He _ Ie _ => exact Or.inr (He.interp_irrel_dep_cast (Ie n Ha rfl))
+    | case Hd _ _ _ Hl Hr Id _ _ _ Il Ir =>  
+      apply Or.inr
       cases HA';
+      rename AnnotSort => k;
+      cases k;
+      case prop => 
+        dsimp only [Stlc.has_dep, Term.stlc] at Ha;
       cases Ha with
-      | inl Ha => exact Id n Ha rfl
+      | inl Ha => exact Hd.interp_irrel_dep_cast (Id n Ha rfl)
       | inr Ha =>
         cases Ha with
         | inl Ha => 
-          cases Il (n + 1) Ha rfl with
+          cases Hl.interp_irrel_dep_cast (Il (n + 1) Ha rfl) with
           | intro A Hv => 
             cases Hv;
             exact ⟨_, by assumption⟩
         | inr Ha => 
-          cases Ir (n + 1) Ha rfl with
+          cases Hr.interp_irrel_dep_cast (Ir (n + 1) Ha rfl) with
           | intro A Hv => 
             cases Hv;
             exact ⟨_, by assumption⟩
-    | elem _ _ _ _ Il _ => exact Il n Ha rfl
-    | let_set _ _ _ _ _ Ie _ _ _ Ie' =>  
+    | elem _ Hl _ _ Il _ => exact Or.inr (Hl.interp_irrel_dep_cast (Il n Ha rfl))
+    | let_set He _ _ _ He' Ie _ _ _ Ie' =>  
+      apply Or.inr
       cases HA';
+      rename AnnotSort => k;
+      cases k;
+      case prop => 
+        dsimp only [Stlc.has_dep, Term.stlc] at Ha;
       cases Ha with
       | inl Ha => 
         cases Ha with
-        | inl Ha => exact Ie n Ha rfl
+        | inl Ha => exact He.interp_irrel_dep_cast (Ie n Ha rfl)
         | inr Ha => cases Ha
       | inr Ha => 
-        cases Ie' (n + 2) Ha rfl with
+        cases He'.interp_irrel_dep_cast (Ie' (n + 2) Ha rfl) with
         | intro A Hv =>
           cases Hv with
           | succ Hv => 
             cases Hv;
             exact ⟨_, by assumption⟩
-    | lam_pr _ _ _ Is => 
-      cases Is (n + 1) Ha rfl with
+    | lam_pr _ Hs _ Is => 
+      cases Hs.interp_irrel_dep_cast (Is (n + 1) Ha rfl) with
       | intro A Hv => 
         cases Hv;
-        exact ⟨_, by assumption⟩
-    | app_pr _ _ _ _ Il _ => 
+        exact Or.inr ⟨_, by assumption⟩
+    | app_pr _ Hl _ _ Il _ => 
       cases Ha with
-      | inl Ha => exact Il n Ha rfl
+      | inl Ha => exact Or.inr (Hl.interp_irrel_dep_cast (Il n Ha rfl))
       | inr Ha => cases Ha
     --TODO: Hmm... the fact that the order is swapped for lam is... interesting...
-    | lam_irrel _ _ _ Is => 
-      cases Is (n + 1) Ha rfl with
+    | lam_irrel _ Hs _ Is => 
+      cases Hs.interp_irrel_dep_cast (Is (n + 1) Ha rfl) with
       | intro A Hv => 
         cases Hv;
-        exact ⟨_, by assumption⟩
-    | app_irrel _ _ _ _ Il _ => 
+        exact Or.inr ⟨_, by assumption⟩
+    | app_irrel _ Hl _ _ Il _ => 
       cases Ha with
-      | inl Ha => exact Il n Ha rfl
+      | inl Ha => exact Or.inr (Hl.interp_irrel_dep_cast (Il n Ha rfl))
       | inr Ha => cases Ha
-    | repr _ _ _ _ _ Ir => exact Ir n Ha rfl
-    | let_repr _ _ _ _ _ Ie _ _ _ Ie' =>  
+    | repr _ _ Hr _ _ Ir => exact Or.inr (Hr.interp_irrel_dep_cast (Ir n Ha rfl))
+    | let_repr He _ _ _ He' Ie _ _ _ Ie' =>  
+      apply Or.inr
       cases HA';
+      rename AnnotSort => k;
+      cases k;
+      case prop => 
+        dsimp only [Stlc.has_dep, Term.stlc] at Ha;
       cases Ha with
       | inl Ha => 
         cases Ha with
         | inl Ha => cases Ha
-        | inr Ha => exact Ie n Ha rfl
+        | inr Ha => exact He.interp_irrel_dep_cast (Ie n Ha rfl)
       | inr Ha => 
-        cases Ie' (n + 2) Ha rfl with
+        cases He'.interp_irrel_dep_cast (Ie' (n + 2) Ha rfl) with
         | intro A Hv =>
           cases Hv with
           | succ Hv => 
             cases Hv;
             exact ⟨_, by assumption⟩
-    | natrec _ _ _ _ _ Ie Iz Is => 
+    | natrec _ He Hz Hs _ Ie Iz Is => 
+      apply Or.inr
       rename AnnotSort => k;
       cases HA';
+      rename AnnotSort => k;
+      cases k;
+      case prop => 
+        dsimp only [Stlc.has_dep, Term.stlc] at Ha;
       cases Ha with
-      | inl Ha => exact Ie n Ha rfl
+      | inl Ha => exact He.interp_irrel_dep_cast (Ie n Ha rfl)
       | inr Ha =>
         cases Ha with
-        | inl Ha => exact Iz n Ha rfl
+        | inl Ha => exact Hz.interp_irrel_dep_cast (Iz n Ha rfl)
         | inr Ha => 
-          cases Is (n + 2) Ha rfl with
+          cases Hs.interp_irrel_dep_cast (Is (n + 2) Ha rfl) with
           | intro A Hv =>
             cases Hv with
             | succ Hv => 
@@ -255,34 +390,54 @@ theorem HasType.interp_irrel_dep {Γ a A}
     | _ => cases HA' <;> cases Ha
   }
 
-theorem HasType.interp_irrel_eq {Γ Δ a A} 
+
+theorem HasType.interp_irrel_dep_ty {Γ a A} 
+  (H: Γ ⊢ a: expr type A) (n: Nat)
+  (Ha: a.stlc.has_dep n): Γ.is_rel n 
+  := H.interp_irrel_dep_cast (H.interp_irrel_dep n Ha)
+
+theorem HasType.interp_irrel_val {Γ a s A} 
+  (H: Γ ⊢ a: expr s A) (n: Nat)
+  (Ha: a.stlc.has_dep n): Γ.is_val n 
+  := match H.interp_irrel_dep n Ha with
+  | Or.inl Ha => by cases Ha; cases H; exact ⟨_, s, by assumption⟩
+  | Or.inr H => by cases H; exact ⟨_, type, by assumption⟩
+
+theorem HasType.interp_irrel_eq_ty {Γ Δ a A} 
   {G: Γ.stlc.interp} {D: Δ.stlc.interp} 
   (HΓ: Γ ⊢ a: expr type A)
   (HΔ: Δ ⊢ a: expr type A)
   (HGD: G.eq_mod_lrt D Γ Δ)
   : G.eq_mod D a.stlc 
   := λ_ Hn => 
-    HGD _ ⟨(HΓ.interp_irrel_dep _ Hn), (HΔ.interp_irrel_dep _ Hn)⟩
+    HGD _ ⟨(HΓ.interp_irrel_dep_ty _ Hn), (HΔ.interp_irrel_dep_ty _ Hn)⟩
 
-theorem HasType.interp_irrel {Γ Δ a A} 
+theorem HasType.interp_irrel_eq {Γ Δ a s A} 
+  {G: Γ.stlc.interp} {D: Δ.stlc.interp} 
+  (HΓ: Γ ⊢ a: expr s A)
+  (HΔ: Δ ⊢ a: expr s A)
+  (HGD: G.eq_mod_lrt_val D Γ Δ)
+  : G.eq_mod D a.stlc 
+  := λ_ Hn => 
+    HGD _ ⟨(HΓ.interp_irrel_val _ Hn), (HΔ.interp_irrel_val _ Hn)⟩
+
+theorem HasType.interp_irrel_ty {Γ Δ a A} 
   {G: Γ.stlc.interp} {D: Δ.stlc.interp} 
   (HΓ: Γ ⊢ a: expr type A)
   (HΔ: Δ ⊢ a: expr type A)
   (HGD: G.eq_mod_lrt D Γ Δ)
   : HΓ.stlc.interp G = HΔ.stlc.interp D
-  := HΓ.stlc.eq_mod HΔ.stlc (HΓ.interp_irrel_eq HΔ HGD)
+  := HΓ.stlc.eq_mod HΔ.stlc (HΓ.interp_irrel_eq_ty HΔ HGD)
 
-theorem HasType.interp_upgrade {Γ a A} 
+theorem HasType.interp_upgrade' {Γ a s A} 
   {G: Γ.upgrade.stlc.interp}
-  (HΓ: Γ ⊢ a: expr type A)
-  (HΔ: Γ.upgrade ⊢ a: expr type A)
+  (HΓ: Γ ⊢ a: expr s A)
+  (HΔ: Γ.upgrade ⊢ a: expr s A)
   : HΓ.stlc.interp G.downgrade = HΔ.stlc.interp G
-  := HΓ.stlc.eq_mod HΔ.stlc 
-    (HΓ.interp_irrel_eq HΔ (G.eq_mod_lrt_downgrade _))
+  := HΓ.stlc.eq_mod HΔ.stlc (HΓ.interp_irrel_eq HΔ (G.eq_mod_lrt_val_downgrade _))
 
-theorem HasType.interp_upgrade' {Γ a A} 
+theorem HasType.interp_upgrade {Γ a s A} 
   {G: Γ.upgrade.stlc.interp}
-  (HΓ: Γ ⊢ a: expr type A)
+  (HΓ: Γ ⊢ a: expr s A)
   : HΓ.stlc.interp G.downgrade = HΓ.upgrade.stlc.interp G
-  := HΓ.stlc.eq_mod HΓ.upgrade.stlc 
-    (HΓ.interp_irrel_eq HΓ.upgrade (G.eq_mod_lrt_downgrade _))
+  := HΓ.interp_upgrade' HΓ.upgrade
