LogicalRefinement/Stlc.lean
@@ -3,7 +3,6 @@ import LogicalRefinement.Stlc.Basic
 import LogicalRefinement.Stlc.Interp
 import LogicalRefinement.Stlc.InterpSubst
 import LogicalRefinement.Stlc.InterpWk
-import LogicalRefinement.Stlc.InterpUpgrade
 import LogicalRefinement.Stlc.InterpIrrel
 import LogicalRefinement.Stlc.Subst
 import LogicalRefinement.Stlc.Irrel
